backend/Tailcallproof.v
@@ -557,7 +557,7 @@ Proof.
   exploit functions_translated; eauto. intro FIND.
   exists (Callstate nil vf vargs2 m2); split.
   setoid_rewrite <- (sig_preserved (Internal f)). econstructor; eauto.
-  constructor; auto. constructor.
+  constructor; auto. constructor. inv H2. auto.
 Qed.
 
 Lemma transf_final_states:
@@ -567,24 +567,24 @@ Proof.
   intros. inv H0. inv H. inv H3.
   eexists; split.
   - constructor.
-  - exists tt. split; constructor; CKLR.uncklr; cbn; auto.
+  - exists (extw m m' H6). split; constructor; CKLR.uncklr; cbn; auto. constructor.
 Qed.
 
 Lemma transf_external_states:
   forall st1 st2 q1, match_states st1 st2 -> at_external ge st1 q1 ->
-  exists q2, at_external tge st2 q2 /\ match_query (cc_c ext) tt q1 q2 /\ se = se /\
-  forall r1 r2 st1', match_reply (cc_c ext) tt r1 r2 -> after_external st1 r1 st1' ->
+  exists w q2, at_external tge st2 q2 /\ match_query (cc_c ext) w q1 q2 /\ se = se /\
+  forall r1 r2 st1', match_reply (cc_c ext) w r1 r2 -> after_external st1 r1 st1' ->
   exists st2', after_external st2 r2 st2' /\ match_states st1' st2'.
 Proof.
   intros st1 st2 q1 Hst Hq1. destruct Hq1. inv Hst.
   exploit functions_translated; eauto. intro FIND'.
-  eexists. intuition idtac.
+  exists (extw m m' H8). eexists. intuition idtac.
   - econstructor; eauto.
   - destruct H6; try discriminate.
-    constructor; CKLR.uncklr; auto.
+    constructor; CKLR.uncklr; auto. constructor.
     destruct v; cbn in *; congruence.
   - inv H1. destruct H0 as ([ ] & [ ] & H0). inv H0. CKLR.uncklr.
-    exists (Returnstate s' vres2 m2'); split; constructor; eauto.
+    exists (Returnstate s' vres2 m2'); split; constructor; eauto. inv H9. auto.
 Qed.
 
 End PRESERVATION.
@@ -601,6 +601,6 @@ Proof.
     eapply (Genv.is_internal_transf_id MATCH). intros [|]; auto.
   - eapply transf_initial_states; eauto.
   - eapply transf_final_states; eauto.
-  - exists tt. eapply transf_external_states; eauto.
+  - eapply transf_external_states; eauto.
   - eapply transf_step_correct; eauto.
 Qed.
